Some progress on ModularInterop.fst

vale/code/arch/x64/interop/ModularInterop.fst
@@ -145,6 +145,32 @@ let wrap code pre post v = fun (x0:M.buffer64) (x1:M.buffer64) ->
   let (stack_b:b8) = LB.alloca (UInt8.uint_to_t 0) (UInt32.uint_to_t 24) in
   lemma_low_assumptions_length stack_b;
   let h2 = HST.get () in
+
+assume (
+  (Seq.equal
+    (LBV.as_seq h0 (LBV.mk_buffer_view (to_b8 x0) Views.view64))
+    (LBV.as_seq h1 (LBV.mk_buffer_view (to_b8 x0) Views.view64))
+  )
+);
+assume (
+  (Seq.equal
+    (LBV.as_seq h1 (LBV.mk_buffer_view (to_b8 x0) Views.view64))
+    (LBV.as_seq h2 (LBV.mk_buffer_view (to_b8 x0) Views.view64))
+  )
+);
+assume (
+  (Seq.equal
+    (LBV.as_seq h0 (LBV.mk_buffer_view (to_b8 x1) Views.view64))
+    (LBV.as_seq h1 (LBV.mk_buffer_view (to_b8 x1) Views.view64))
+  )
+);
+assume (
+  (Seq.equal
+    (LBV.as_seq h1 (LBV.mk_buffer_view (to_b8 x1) Views.view64))
+    (LBV.as_seq h2 (LBV.mk_buffer_view (to_b8 x1) Views.view64))
+  )
+);
+
   assert (HS.fresh_frame h0 h1);
   assert (disjoint_or_eq_l_aux x0 []);
   assert (disjoint_or_eq_l_aux x0 [x1]);
@@ -178,7 +204,7 @@ let wrap code pre post v = fun (x0:M.buffer64) (x1:M.buffer64) ->
     assert (LB.live h0' stack_b);
     let va_mem = va_s0.VS.mem in
     let num_stack_slots = 3 in
-    assume (low_assumptions h0 va_mem x0 x1);
+    assert (low_assumptions h0 va_mem x0 x1);
     assert_norm (List.memP x0 [stack_b; x0; x1]);
     assert_norm (List.memP x1 [stack_b; x0; x1]);
     assert (M.buffer_readable va_mem x0);
@@ -199,9 +225,21 @@ let wrap code pre post v = fun (x0:M.buffer64) (x1:M.buffer64) ->
   assert (LB.modifies (LB.loc_union (LB.loc_buffer (to_b8 stack_b)) (LB.loc_union (LB.loc_buffer (to_b8 x0)) (LB.loc_buffer (to_b8 x1)))) h2 h3);
   HST.pop_frame ();
   let h4 = HST.get () in
+assume (
+  (Seq.equal
+    (LBV.as_seq h3 (LBV.mk_buffer_view (to_b8 x0) Views.view64))
+    (LBV.as_seq h4 (LBV.mk_buffer_view (to_b8 x0) Views.view64))
+  )
+);
+assume (
+  (Seq.equal
+    (LBV.as_seq h3 (LBV.mk_buffer_view (to_b8 x1) Views.view64))
+    (LBV.as_seq h4 (LBV.mk_buffer_view (to_b8 x1) Views.view64))
+  )
+);
   assert (LB.modifies (LB.loc_union (LB.loc_buffer (to_b8 x0)) (LB.loc_buffer (to_b8 x1))) h0 h4);
   assert (low_assumptions h0 va_s0.VS.mem x0 x1);
-  assume (low_assumptions h4 va_s1.VS.mem x0 x1);
+  assert (low_assumptions h4 va_s1.VS.mem x0 x1);
   assert (post IA.win x0 x1 va_s0 stack_b va_s1 fuel);
   assert (to_low_post post x0 x1 h0 () h4);
   ()
